<?xml version="1.0"?>
<rdf:RDF xmlns="http://lod.ehri-project-test.eu/ontology#"
     xml:base="http://lod.ehri-project-test.eu/ontology"
     xmlns:dc="http://purl.org/dc/elements/1.1/"
     xmlns:ns="http://creativecommons.org/ns#"
     xmlns:owl="http://www.w3.org/2002/07/owl#"
     xmlns:rdf="http://www.w3.org/1999/02/22-rdf-syntax-ns#"
     xmlns:xml="http://www.w3.org/XML/1998/namespace"
     xmlns:xsd="http://www.w3.org/2001/XMLSchema#"
     xmlns:ehri="http://lod.ehri-project-test.eu/ontology#"
     xmlns:foaf="http://xmlns.com/foaf/0.1/"
     xmlns:rdfs="http://www.w3.org/2000/01/rdf-schema#"
     xmlns:rico="https://www.ica.org/standards/RiC/ontology#"
     xmlns:skos="http://www.w3.org/2004/02/skos/core#"
     xmlns:vann="http://purl.org/vocab/vann/"
     xmlns:terms="http://purl.org/dc/terms/"
     xmlns:schema="http://schema.org/">
    <owl:Ontology rdf:about="http://lod.ehri-project-test.eu/ontology">
        <owl:versionIRI rdf:resource="http://lod.ehri-project-test.eu/ontology/0.0.1"/>
        <owl:imports rdf:resource="https://www.ica.org/standards/RiC/ontology/1.0.2"/>
        <ns:license rdf:resource="https://creativecommons.org/licenses/by/4.0/"/>
        <dc:creator xml:lang="en">Herminio García-González (Kazerne Dossin)</dc:creator>
        <dc:creator xml:lang="en">Mike Bryant (NIOD)</dc:creator>
        <dc:title xml:lang="en">EHRI Ontology</dc:title>
        <terms:abstract xml:lang="en">This ontology defines the data model used by the EHRI-KG for the representation of the information hosted in the EHRI Portal. It does so by extending RiC-O v1.0.2 and reusing some of the schema.org concepts.</terms:abstract>
        <terms:description xml:lang="en">The EHRI Ontology extends some of the RiC-O types and foremostly adds new properties to represent all the data present in the EHRI Portal. Whenever a class is extended with new properties, a subclass bounded to the ehri prefix is created in order to preserve the original RiC-O axioms intact. In other cases, some classes are specialised and subclasses add more meaning to the superclass.</terms:description>
        <terms:publisher>EHRI-ERIC</terms:publisher>
        <vann:preferredNamespacePrefix>ehri</vann:preferredNamespacePrefix>
        <vann:preferredNamespaceUri rdf:resource="http://lod.ehri-project-test.eu/ontology#"/>
        <schema:codeRepository rdf:resource="https://github.com/EHRI/ehri-kg-ontology"/>
        <owl:versionInfo>v0.0.1</owl:versionInfo>
        <foaf:logo rdf:resource="https://ehri-kg.ehri-project.eu/images/ehri-logo.svg"/>
    </owl:Ontology>
    


    <!-- 
    ///////////////////////////////////////////////////////////////////////////////////////
    //
    // Annotation properties
    //
    ///////////////////////////////////////////////////////////////////////////////////////
     -->

    


    <!-- http://purl.org/dc/elements/1.1/contributor -->

    <owl:AnnotationProperty rdf:about="http://purl.org/dc/elements/1.1/contributor">
        <rdfs:subPropertyOf rdf:resource="http://www.w3.org/2000/01/rdf-schema#comment"/>
    </owl:AnnotationProperty>
    


    <!-- http://purl.org/vocab/vann/preferredNamespacePrefix -->

    <owl:AnnotationProperty rdf:about="http://purl.org/vocab/vann/preferredNamespacePrefix"/>
    


    <!-- http://purl.org/vocab/vann/preferredNamespaceUri -->

    <owl:AnnotationProperty rdf:about="http://purl.org/vocab/vann/preferredNamespaceUri"/>
    


    <!-- http://schema.org/codeRepository -->

    <owl:AnnotationProperty rdf:about="http://schema.org/codeRepository"/>
    


    <!-- http://www.w3.org/2004/02/skos/core#definition -->

    <owl:AnnotationProperty rdf:about="http://www.w3.org/2004/02/skos/core#definition"/>
    


    <!-- http://xmlns.com/foaf/0.1/logo -->

    <owl:AnnotationProperty rdf:about="http://xmlns.com/foaf/0.1/logo"/>
    


    <!-- 
    ///////////////////////////////////////////////////////////////////////////////////////
    //
    // Object Properties
    //
    ///////////////////////////////////////////////////////////////////////////////////////
     -->

    


    <!-- http://lod.ehri-project-test.eu/ontology#hasCopy -->

    <owl:ObjectProperty rdf:about="http://lod.ehri-project-test.eu/ontology#hasCopy">
        <rdfs:subPropertyOf rdf:resource="https://www.ica.org/standards/RiC/ontology#hasCopy"/>
        <rdfs:subPropertyOf rdf:resource="https://www.ica.org/standards/RiC/ontology#isRelatedTo"/>
        <owl:inverseOf rdf:resource="http://lod.ehri-project-test.eu/ontology#isCopyOf"/>
        <rdfs:domain>
            <owl:Class>
                <owl:unionOf rdf:parseType="Collection">
                    <rdf:Description rdf:about="http://lod.ehri-project-test.eu/ontology#Institution"/>
                    <rdf:Description rdf:about="http://lod.ehri-project-test.eu/ontology#RecordResource"/>
                </owl:unionOf>
            </owl:Class>
        </rdfs:domain>
        <rdfs:range>
            <owl:Class>
                <owl:unionOf rdf:parseType="Collection">
                    <rdf:Description rdf:about="http://lod.ehri-project-test.eu/ontology#Institution"/>
                    <rdf:Description rdf:about="http://lod.ehri-project-test.eu/ontology#RecordResource"/>
                </owl:unionOf>
            </owl:Class>
        </rdfs:range>
        <rdfs:comment xml:lang="en">This is a generalisation of the rico:hasCopy property to expand the domain and range to ehri:Institution instances.</rdfs:comment>
        <rdfs:label xml:lang="fr">a pour copie</rdfs:label>
        <rdfs:label xml:lang="en">has copy</rdfs:label>
        <rdfs:label xml:lang="es">tiene como copia</rdfs:label>
    </owl:ObjectProperty>
    


    <!-- http://lod.ehri-project-test.eu/ontology#isCopyOf -->

    <owl:ObjectProperty rdf:about="http://lod.ehri-project-test.eu/ontology#isCopyOf">
        <rdfs:subPropertyOf rdf:resource="https://www.ica.org/standards/RiC/ontology#isCopyOf"/>
        <rdfs:subPropertyOf rdf:resource="https://www.ica.org/standards/RiC/ontology#isRelatedTo"/>
        <rdfs:domain>
            <owl:Class>
                <owl:unionOf rdf:parseType="Collection">
                    <rdf:Description rdf:about="http://lod.ehri-project-test.eu/ontology#Institution"/>
                    <rdf:Description rdf:about="http://lod.ehri-project-test.eu/ontology#RecordResource"/>
                </owl:unionOf>
            </owl:Class>
        </rdfs:domain>
        <rdfs:range>
            <owl:Class>
                <owl:unionOf rdf:parseType="Collection">
                    <rdf:Description rdf:about="http://lod.ehri-project-test.eu/ontology#Institution"/>
                    <rdf:Description rdf:about="http://lod.ehri-project-test.eu/ontology#RecordResource"/>
                </owl:unionOf>
            </owl:Class>
        </rdfs:range>
        <rdfs:comment xml:lang="en">Inverse of ehri:hasCopy object property.</rdfs:comment>
        <rdfs:label xml:lang="es">es copia de</rdfs:label>
        <rdfs:label xml:lang="fr">est la copie de</rdfs:label>
        <rdfs:label xml:lang="en">is copy of</rdfs:label>
    </owl:ObjectProperty>
    


    <!-- http://lod.ehri-project-test.eu/ontology#scriptOfMaterials -->

    <owl:ObjectProperty rdf:about="http://lod.ehri-project-test.eu/ontology#scriptOfMaterials">
        <rdfs:subPropertyOf rdf:resource="https://www.ica.org/standards/RiC/ontology#isRelatedTo"/>
        <rdfs:domain rdf:resource="http://lod.ehri-project-test.eu/ontology#RecordResource"/>
        <rdfs:range rdf:resource="http://lod.ehri-project-test.eu/ontology#MaterialScript"/>
        <rdfs:comment xml:lang="en">This property allows to indicate the script present in the materials</rdfs:comment>
        <rdfs:label xml:lang="es">la documentación tiene o tenía como escritura</rdfs:label>
        <rdfs:label xml:lang="fr">la documentation a ou a eu pour écriture</rdfs:label>
        <rdfs:label xml:lang="en">materials have or had script</rdfs:label>
    </owl:ObjectProperty>
    


    <!-- 
    ///////////////////////////////////////////////////////////////////////////////////////
    //
    // Data properties
    //
    ///////////////////////////////////////////////////////////////////////////////////////
     -->

    


    <!-- http://lod.ehri-project-test.eu/ontology#accessibility -->

    <owl:DatatypeProperty rdf:about="http://lod.ehri-project-test.eu/ontology#accessibility">
        <rdfs:domain rdf:resource="http://lod.ehri-project-test.eu/ontology#Institution"/>
        <rdfs:range rdf:resource="http://www.w3.org/2000/01/rdf-schema#Literal"/>
        <rdfs:comment xml:lang="en">Collects information about the institution&apos;s accesibility with respect to its archival holdings and services.</rdfs:comment>
        <rdfs:label xml:lang="es">accesibilidad</rdfs:label>
        <rdfs:label xml:lang="en">accessibility</rdfs:label>
        <rdfs:label xml:lang="fr">accessibilité</rdfs:label>
    </owl:DatatypeProperty>
    


    <!-- http://lod.ehri-project-test.eu/ontology#administrativeStructure -->

    <owl:DatatypeProperty rdf:about="http://lod.ehri-project-test.eu/ontology#administrativeStructure">
        <rdfs:domain rdf:resource="http://lod.ehri-project-test.eu/ontology#Institution"/>
        <rdfs:range rdf:resource="http://www.w3.org/2000/01/rdf-schema#Literal"/>
        <rdfs:comment xml:lang="en">Represents the current administrative structure of an institution.</rdfs:comment>
        <rdfs:label xml:lang="en">administrative structure</rdfs:label>
        <rdfs:label xml:lang="es">estructura administrativa</rdfs:label>
        <rdfs:label xml:lang="fr">structure administrative</rdfs:label>
    </owl:DatatypeProperty>
    


    <!-- http://lod.ehri-project-test.eu/ontology#appraisal -->

    <owl:DatatypeProperty rdf:about="http://lod.ehri-project-test.eu/ontology#appraisal">
        <rdfs:domain rdf:resource="http://lod.ehri-project-test.eu/ontology#Record"/>
        <rdfs:range rdf:resource="http://www.w3.org/2000/01/rdf-schema#Literal"/>
        <rdfs:comment xml:lang="en">Provides information on any appraisal, destruction and scheduling action.</rdfs:comment>
        <rdfs:label xml:lang="en">appraisal</rdfs:label>
        <rdfs:label xml:lang="es">valoración</rdfs:label>
        <rdfs:label xml:lang="fr">évaluation</rdfs:label>
    </owl:DatatypeProperty>
    


    <!-- http://lod.ehri-project-test.eu/ontology#archivalHistory -->

    <owl:DatatypeProperty rdf:about="http://lod.ehri-project-test.eu/ontology#archivalHistory">
        <rdfs:subPropertyOf rdf:resource="https://www.ica.org/standards/RiC/ontology#history"/>
        <rdfs:domain rdf:resource="http://lod.ehri-project-test.eu/ontology#Country"/>
        <rdfs:range rdf:resource="http://www.w3.org/2000/01/rdf-schema#Literal"/>
        <rdfs:comment xml:lang="en">Holds information about the Holocaust and WWII and how it relates to the archival landscape in that country.</rdfs:comment>
        <rdfs:label xml:lang="en">archival history</rdfs:label>
        <rdfs:label xml:lang="fr">histoire archivistique</rdfs:label>
        <rdfs:label xml:lang="es">historia archivística</rdfs:label>
    </owl:DatatypeProperty>
    


    <!-- http://lod.ehri-project-test.eu/ontology#archivalSituation -->

    <owl:DatatypeProperty rdf:about="http://lod.ehri-project-test.eu/ontology#archivalSituation">
        <rdfs:domain rdf:resource="http://lod.ehri-project-test.eu/ontology#Country"/>
        <rdfs:range rdf:resource="http://www.w3.org/2000/01/rdf-schema#Literal"/>
        <rdfs:comment xml:lang="en">Offers a short introduction to the archival situation and culture in a country.</rdfs:comment>
        <rdfs:label xml:lang="en">archival situation</rdfs:label>
        <rdfs:label xml:lang="es">situación de los archivos</rdfs:label>
        <rdfs:label xml:lang="fr">situation de conservation</rdfs:label>
    </owl:DatatypeProperty>
    


    <!-- http://lod.ehri-project-test.eu/ontology#archivistNote -->

    <owl:DatatypeProperty rdf:about="http://lod.ehri-project-test.eu/ontology#archivistNote">
        <rdfs:subPropertyOf rdf:resource="http://lod.ehri-project-test.eu/ontology#notes"/>
        <rdfs:domain rdf:resource="http://lod.ehri-project-test.eu/ontology#RecordResource"/>
        <rdfs:range rdf:resource="http://www.w3.org/2000/01/rdf-schema#Literal"/>
        <rdfs:comment xml:lang="en">Explains how the description was prepared and by whom.</rdfs:comment>
        <rdfs:label xml:lang="en">archivist note</rdfs:label>
        <rdfs:label xml:lang="es">nota del archivero/a</rdfs:label>
        <rdfs:label xml:lang="fr">notes de l&apos;archiviste</rdfs:label>
    </owl:DatatypeProperty>
    


    <!-- http://lod.ehri-project-test.eu/ontology#buildings -->

    <owl:DatatypeProperty rdf:about="http://lod.ehri-project-test.eu/ontology#buildings">
        <rdfs:domain rdf:resource="http://lod.ehri-project-test.eu/ontology#Institution"/>
        <rdfs:range rdf:resource="http://www.w3.org/2000/01/rdf-schema#Literal"/>
        <rdfs:comment xml:lang="en">Provides information about the buildings of the institution</rdfs:comment>
        <rdfs:label xml:lang="en">building(s)</rdfs:label>
        <rdfs:label xml:lang="fr">bâtiment(s)</rdfs:label>
        <rdfs:label xml:lang="es">edificio(s)</rdfs:label>
    </owl:DatatypeProperty>
    


    <!-- http://lod.ehri-project-test.eu/ontology#contactPerson -->

    <owl:DatatypeProperty rdf:about="http://lod.ehri-project-test.eu/ontology#contactPerson">
        <rdfs:domain rdf:resource="http://lod.ehri-project-test.eu/ontology#InstitutionAddress"/>
        <rdfs:range rdf:resource="http://www.w3.org/2000/01/rdf-schema#Literal"/>
        <rdfs:comment xml:lang="en">To provide the information needed to contact members of the staff.</rdfs:comment>
        <rdfs:label xml:lang="en">contact person</rdfs:label>
        <rdfs:label xml:lang="es">persona de contacto</rdfs:label>
        <rdfs:label xml:lang="fr">personne de contact</rdfs:label>
    </owl:DatatypeProperty>
    


    <!-- http://lod.ehri-project-test.eu/ontology#findingAids -->

    <owl:DatatypeProperty rdf:about="http://lod.ehri-project-test.eu/ontology#findingAids">
        <rdfs:domain rdf:resource="http://lod.ehri-project-test.eu/ontology#Institution"/>
        <rdfs:range rdf:resource="http://www.w3.org/2000/01/rdf-schema#Literal"/>
        <rdfs:comment xml:lang="en">Provides a general overview of the published and/or published finding aids.</rdfs:comment>
        <rdfs:label xml:lang="en">finding aids</rdfs:label>
        <rdfs:label xml:lang="es">instrumentos de descripción</rdfs:label>
        <rdfs:label xml:lang="fr">instruments de recherche</rdfs:label>
    </owl:DatatypeProperty>
    


    <!-- http://lod.ehri-project-test.eu/ontology#generalContext -->

    <owl:DatatypeProperty rdf:about="http://lod.ehri-project-test.eu/ontology#generalContext">
        <rdfs:subPropertyOf rdf:resource="https://www.ica.org/standards/RiC/ontology#generalDescription"/>
        <rdfs:domain rdf:resource="http://lod.ehri-project-test.eu/ontology#Institution"/>
        <rdfs:range rdf:resource="http://www.w3.org/2000/01/rdf-schema#Literal"/>
        <rdfs:comment xml:lang="en">Provides information about the geographical and cultural context of the institution.</rdfs:comment>
        <rdfs:label xml:lang="fr">contexte général</rdfs:label>
        <rdfs:label xml:lang="es">contexto general</rdfs:label>
        <rdfs:label xml:lang="en">general context</rdfs:label>
    </owl:DatatypeProperty>
    


    <!-- http://lod.ehri-project-test.eu/ontology#institutionConditionsOfAccess -->

    <owl:DatatypeProperty rdf:about="http://lod.ehri-project-test.eu/ontology#institutionConditionsOfAccess">
        <rdfs:domain rdf:resource="http://lod.ehri-project-test.eu/ontology#Institution"/>
        <rdfs:range rdf:resource="http://www.w3.org/2000/01/rdf-schema#Literal"/>
        <rdfs:comment xml:lang="en">Collects information about the conditions, requirements and procedures for access to, and use of institutional services</rdfs:comment>
        <rdfs:label xml:lang="es">condiciones de acceso de una institución</rdfs:label>
        <rdfs:label xml:lang="fr">conditions d&apos;accès d&apos;une institution</rdfs:label>
        <rdfs:label xml:lang="en">conditions of access of an institution</rdfs:label>
    </owl:DatatypeProperty>
    


    <!-- http://lod.ehri-project-test.eu/ontology#institutionReproductionServices -->

    <owl:DatatypeProperty rdf:about="http://lod.ehri-project-test.eu/ontology#institutionReproductionServices">
        <rdfs:domain rdf:resource="http://lod.ehri-project-test.eu/ontology#Institution"/>
        <rdfs:range rdf:resource="http://www.w3.org/2000/01/rdf-schema#Literal"/>
        <rdfs:comment xml:lang="en">Gather information on the legal status or other regulations that restrict or affect access to the unit of description.</rdfs:comment>
        <rdfs:label xml:lang="en">reproduction services</rdfs:label>
        <rdfs:label xml:lang="fr">services de reproduction</rdfs:label>
        <rdfs:label xml:lang="es">servicios de reproducción</rdfs:label>
    </owl:DatatypeProperty>
    


    <!-- http://lod.ehri-project-test.eu/ontology#locationOfCopies -->

    <owl:DatatypeProperty rdf:about="http://lod.ehri-project-test.eu/ontology#locationOfCopies">
        <rdfs:domain rdf:resource="http://lod.ehri-project-test.eu/ontology#RecordResource"/>
        <rdfs:range rdf:resource="http://www.w3.org/2000/01/rdf-schema#Literal"/>
        <rdfs:comment xml:lang="en">Indicates the existence, location and availability of copies of the unit of description.</rdfs:comment>
        <rdfs:label xml:lang="en">existence and location of copies</rdfs:label>
        <rdfs:label xml:lang="fr">existence et lieu de copies</rdfs:label>
        <rdfs:label xml:lang="es">existencia y localización de copias</rdfs:label>
    </owl:DatatypeProperty>
    


    <!-- http://lod.ehri-project-test.eu/ontology#locationOfOriginals -->

    <owl:DatatypeProperty rdf:about="http://lod.ehri-project-test.eu/ontology#locationOfOriginals">
        <rdfs:domain rdf:resource="http://lod.ehri-project-test.eu/ontology#RecordResource"/>
        <rdfs:range rdf:resource="http://www.w3.org/2000/01/rdf-schema#Literal"/>
        <rdfs:comment xml:lang="en">Indicates the existence, location, availability and/or destruction of originals where the unit of description consists of copies.</rdfs:comment>
        <rdfs:label xml:lang="en">existence and location of originals</rdfs:label>
        <rdfs:label xml:lang="fr">existence et lieu des originaux</rdfs:label>
        <rdfs:label xml:lang="es">existencia y localización de los originales</rdfs:label>
    </owl:DatatypeProperty>
    


    <!-- http://lod.ehri-project-test.eu/ontology#notes -->

    <owl:DatatypeProperty rdf:about="http://lod.ehri-project-test.eu/ontology#notes">
        <rdfs:domain rdf:resource="http://lod.ehri-project-test.eu/ontology#RecordResource"/>
        <rdfs:range rdf:resource="http://www.w3.org/2000/01/rdf-schema#Literal"/>
        <rdfs:comment xml:lang="en">Provides information that cannot be accommodated in any of the other data properties</rdfs:comment>
        <rdfs:label xml:lang="es">nota(s)</rdfs:label>
        <rdfs:label xml:lang="en">note(s)</rdfs:label>
        <rdfs:label xml:lang="fr">note(s)</rdfs:label>
    </owl:DatatypeProperty>
    


    <!-- http://lod.ehri-project-test.eu/ontology#otherFindingAids -->

    <owl:DatatypeProperty rdf:about="http://lod.ehri-project-test.eu/ontology#otherFindingAids">
        <rdfs:domain rdf:resource="http://lod.ehri-project-test.eu/ontology#RecordResource"/>
        <rdfs:range rdf:resource="http://www.w3.org/2000/01/rdf-schema#Literal"/>
        <rdfs:comment xml:lang="en">Provide information on the history of the unit of description that is significant for its authenticity, integrity and interpretation.</rdfs:comment>
        <rdfs:label xml:lang="fr">autres instruments de recherche</rdfs:label>
        <rdfs:label xml:lang="en">other finding aids</rdfs:label>
        <rdfs:label xml:lang="es">otros instrumentos de descripción</rdfs:label>
    </owl:DatatypeProperty>
    


    <!-- http://lod.ehri-project-test.eu/ontology#physicalCharacterisiticsAndTechnicalRequirements -->

    <owl:DatatypeProperty rdf:about="http://lod.ehri-project-test.eu/ontology#physicalCharacterisiticsAndTechnicalRequirements">
        <rdfs:domain rdf:resource="http://lod.ehri-project-test.eu/ontology#RecordResource"/>
        <rdfs:range rdf:resource="http://www.w3.org/2000/01/rdf-schema#Literal"/>
        <rdfs:comment xml:lang="en">Collects information about any important physical characteristics or technical requirements that affect use of the unit of description.</rdfs:comment>
        <rdfs:label xml:lang="es">características físicas y requisitos técnicos</rdfs:label>
        <rdfs:label xml:lang="fr">caractéristiques matérielles et contraintes techniques</rdfs:label>
        <rdfs:label xml:lang="en">physical characteristics and technical requirements</rdfs:label>
    </owl:DatatypeProperty>
    


    <!-- http://lod.ehri-project-test.eu/ontology#publicAreas -->

    <owl:DatatypeProperty rdf:about="http://lod.ehri-project-test.eu/ontology#publicAreas">
        <rdfs:domain rdf:resource="http://lod.ehri-project-test.eu/ontology#Institution"/>
        <rdfs:range rdf:resource="http://www.w3.org/2000/01/rdf-schema#Literal"/>
        <rdfs:comment xml:lang="en">Collects information about areas of the institution available for public use.</rdfs:comment>
        <rdfs:label xml:lang="fr">espaces publics</rdfs:label>
        <rdfs:label xml:lang="es">espacios públicos</rdfs:label>
        <rdfs:label xml:lang="en">public areas</rdfs:label>
    </owl:DatatypeProperty>
    


    <!-- http://lod.ehri-project-test.eu/ontology#recordsManagementAndCollectingPolicies -->

    <owl:DatatypeProperty rdf:about="http://lod.ehri-project-test.eu/ontology#recordsManagementAndCollectingPolicies">
        <rdfs:domain rdf:resource="http://lod.ehri-project-test.eu/ontology#Institution"/>
        <rdfs:range rdf:resource="http://www.w3.org/2000/01/rdf-schema#Literal"/>
        <rdfs:comment xml:lang="en">Provides information about the records management and collecting policies of the institution with archival holdings.</rdfs:comment>
        <rdfs:label xml:lang="fr">gestion des archives courantes et intermédiaires et politiques de collecte</rdfs:label>
        <rdfs:label xml:lang="es">gestión de documentos y política de ingresos</rdfs:label>
        <rdfs:label xml:lang="en">records management and collecting policies</rdfs:label>
    </owl:DatatypeProperty>
    


    <!-- http://lod.ehri-project-test.eu/ontology#relatedMaterial -->

    <owl:DatatypeProperty rdf:about="http://lod.ehri-project-test.eu/ontology#relatedMaterial">
        <rdfs:domain rdf:resource="http://lod.ehri-project-test.eu/ontology#RecordResource"/>
        <rdfs:range rdf:resource="http://www.w3.org/2000/01/rdf-schema#Literal"/>
        <rdfs:comment xml:lang="en">Identifies related units of description.</rdfs:comment>
        <rdfs:label xml:lang="en">related units of description</rdfs:label>
        <rdfs:label xml:lang="fr">sources complémentaires</rdfs:label>
        <rdfs:label xml:lang="es">unidades de descripción relacionadas</rdfs:label>
    </owl:DatatypeProperty>
    


    <!-- http://lod.ehri-project-test.eu/ontology#researchExtensive -->

    <owl:DatatypeProperty rdf:about="http://lod.ehri-project-test.eu/ontology#researchExtensive">
        <rdfs:domain rdf:resource="http://lod.ehri-project-test.eu/ontology#Country"/>
        <rdfs:range rdf:resource="http://www.w3.org/2000/01/rdf-schema#Literal"/>
        <rdfs:comment xml:lang="en">Offers information on how EHRI acquiered its data and integrated it into the Portal.</rdfs:comment>
        <rdfs:label xml:lang="es">investigación del EHRI (ampliado)</rdfs:label>
        <rdfs:label xml:lang="fr">recherche par EHRI (extensif)</rdfs:label>
        <rdfs:label xml:lang="en">research by EHRI (extensive)</rdfs:label>
    </owl:DatatypeProperty>
    


    <!-- http://lod.ehri-project-test.eu/ontology#researchServices -->

    <owl:DatatypeProperty rdf:about="http://lod.ehri-project-test.eu/ontology#researchServices">
        <rdfs:domain rdf:resource="http://lod.ehri-project-test.eu/ontology#Institution"/>
        <rdfs:range rdf:resource="http://www.w3.org/2000/01/rdf-schema#Literal"/>
        <rdfs:comment xml:lang="en">Describes the research services provided by the institution with archival holdings.</rdfs:comment>
        <rdfs:label xml:lang="en">research services</rdfs:label>
        <rdfs:label xml:lang="fr">services d&apos;aide à la recherche</rdfs:label>
        <rdfs:label xml:lang="es">servicios de ayuda a la investigación</rdfs:label>
    </owl:DatatypeProperty>
    


    <!-- http://lod.ehri-project-test.eu/ontology#researchSummary -->

    <owl:DatatypeProperty rdf:about="http://lod.ehri-project-test.eu/ontology#researchSummary">
        <rdfs:domain rdf:resource="http://lod.ehri-project-test.eu/ontology#Country"/>
        <rdfs:range rdf:resource="http://www.w3.org/2000/01/rdf-schema#Literal"/>
        <rdfs:comment xml:lang="en">Elaborates on EHRI&apos;s identification work, which is ongoing since October 2010. This section also includes references to aggregators and country-specific research guides.</rdfs:comment>
        <rdfs:label xml:lang="es">investigación del EHRI (resumen)</rdfs:label>
        <rdfs:label xml:lang="fr">recherche EHRI (récapitulatif)</rdfs:label>
        <rdfs:label xml:lang="en">research by EHRI (summary)</rdfs:label>
    </owl:DatatypeProperty>
    


    <!-- http://lod.ehri-project-test.eu/ontology#separatedMaterial -->

    <owl:DatatypeProperty rdf:about="http://lod.ehri-project-test.eu/ontology#separatedMaterial">
        <rdfs:domain rdf:resource="http://lod.ehri-project-test.eu/ontology#RecordResource"/>
        <rdfs:range rdf:resource="http://www.w3.org/2000/01/rdf-schema#Literal"/>
        <rdfs:comment xml:lang="en">Information about materials that are associated by provenance to the described materials but that have been physically separated or removed. Items may be separated for various reasons, including the dispersal of special formats to more appropriate custodial units; the outright destruction of duplicate or nonessential material; and the deliberate or unintentional scattering of fonds among different repositories.</rdfs:comment>
        <rdfs:label xml:lang="en">separated units of description</rdfs:label>
        <rdfs:label xml:lang="fr">sources séparées</rdfs:label>
        <rdfs:label xml:lang="es">unidadades de descripción separadas</rdfs:label>
    </owl:DatatypeProperty>
    


    <!-- http://lod.ehri-project-test.eu/ontology#sources -->

    <owl:DatatypeProperty rdf:about="http://lod.ehri-project-test.eu/ontology#sources">
        <rdfs:domain>
            <owl:Class>
                <owl:unionOf rdf:parseType="Collection">
                    <rdf:Description rdf:about="http://lod.ehri-project-test.eu/ontology#RecordResource"/>
                    <rdf:Description rdf:about="https://www.ica.org/standards/RiC/ontology#Agent"/>
                </owl:unionOf>
            </owl:Class>
        </rdfs:domain>
        <rdfs:range rdf:resource="http://www.w3.org/2000/01/rdf-schema#Literal"/>
        <rdfs:comment xml:lang="en">Record notes on sources consulted in preparing the description and who prepared it.</rdfs:comment>
        <rdfs:label xml:lang="es">fuentes</rdfs:label>
        <rdfs:label xml:lang="en">sources</rdfs:label>
        <rdfs:label xml:lang="fr">sources</rdfs:label>
    </owl:DatatypeProperty>
    


    <!-- http://lod.ehri-project-test.eu/ontology#structureOrGenealogy -->

    <owl:DatatypeProperty rdf:about="http://lod.ehri-project-test.eu/ontology#structureOrGenealogy">
        <rdfs:domain rdf:resource="https://www.ica.org/standards/RiC/ontology#Agent"/>
        <rdfs:range rdf:resource="http://www.w3.org/2000/01/rdf-schema#Literal"/>
        <rdfs:comment xml:lang="en">Describes and/or represents the internal administrative structure(s) of a corporate body or the genealogy of a family.</rdfs:comment>
        <rdfs:label xml:lang="es">estructura(s) interna(s)/genealogía</rdfs:label>
        <rdfs:label xml:lang="en">internal structure</rdfs:label>
        <rdfs:label xml:lang="fr">structure interne</rdfs:label>
    </owl:DatatypeProperty>
    


    <!-- http://lod.ehri-project-test.eu/ontology#wasUsedAsSourceIn -->

    <owl:DatatypeProperty rdf:about="http://lod.ehri-project-test.eu/ontology#wasUsedAsSourceIn">
        <rdfs:domain rdf:resource="http://lod.ehri-project-test.eu/ontology#RecordResource"/>
        <rdfs:range rdf:resource="http://www.w3.org/2000/01/rdf-schema#Literal"/>
        <rdfs:comment xml:lang="en">Identifies any publications that are about or are based on the use, study, or analysis of the unit of description.</rdfs:comment>
        <rdfs:label xml:lang="fr">bibliographie</rdfs:label>
        <rdfs:label xml:lang="es">nota de publicaciones</rdfs:label>
        <rdfs:label xml:lang="en">publication note</rdfs:label>
    </owl:DatatypeProperty>
    


    <!-- http://schema.org/contactType -->

    <owl:DatatypeProperty rdf:about="http://schema.org/contactType">
        <rdfs:domain rdf:resource="http://schema.org/PostalAddress"/>
        <rdfs:range rdf:resource="http://www.w3.org/2000/01/rdf-schema#Literal"/>
        <rdfs:comment xml:lang="en">A person or organization can have different contact points, for different purposes. For example, a sales contact point, a PR contact point and so on. This property is used to specify the kind of contact point.</rdfs:comment>
        <rdfs:isDefinedBy rdf:resource="http://schema.org/contactType"/>
        <rdfs:label xml:lang="en">contact type</rdfs:label>
        <rdfs:label xml:lang="es">tipo de contacto</rdfs:label>
        <rdfs:label xml:lang="fr">type de contact</rdfs:label>
    </owl:DatatypeProperty>
    


    <!-- http://schema.org/email -->

    <owl:DatatypeProperty rdf:about="http://schema.org/email">
        <rdfs:domain rdf:resource="http://schema.org/PostalAddress"/>
        <rdfs:range rdf:resource="http://www.w3.org/2000/01/rdf-schema#Literal"/>
        <rdfs:comment xml:lang="en">Email address.</rdfs:comment>
        <rdfs:isDefinedBy rdf:resource="http://schema.org/email"/>
        <rdfs:label xml:lang="fr">adresse email</rdfs:label>
        <rdfs:label xml:lang="es">dirección de correo electrónico</rdfs:label>
        <rdfs:label xml:lang="en">email address</rdfs:label>
    </owl:DatatypeProperty>
    


    <!-- http://schema.org/faxNumber -->

    <owl:DatatypeProperty rdf:about="http://schema.org/faxNumber">
        <rdfs:domain rdf:resource="http://schema.org/PostalAddress"/>
        <rdfs:range rdf:resource="http://www.w3.org/2000/01/rdf-schema#Literal"/>
        <rdfs:comment xml:lang="en">The fax number.</rdfs:comment>
        <rdfs:isDefinedBy rdf:resource="http://schema.org/faxNumber"/>
        <rdfs:label xml:lang="en">fax number</rdfs:label>
        <rdfs:label xml:lang="fr">numéro de fax</rdfs:label>
        <rdfs:label xml:lang="es">número de fax</rdfs:label>
    </owl:DatatypeProperty>
    


    <!-- http://schema.org/openingHours -->

    <owl:DatatypeProperty rdf:about="http://schema.org/openingHours">
        <rdfs:domain rdf:resource="http://schema.org/ArchiveOrganization"/>
        <rdfs:range rdf:resource="http://www.w3.org/2000/01/rdf-schema#Literal"/>
        <rdfs:comment xml:lang="en">The general opening hours for a business.</rdfs:comment>
        <rdfs:label rdf:resource="http://schema.org/openingHours"/>
        <rdfs:label xml:lang="fr">heures d&apos;ouverture</rdfs:label>
        <rdfs:label xml:lang="es">horarios de apertura</rdfs:label>
        <rdfs:label xml:lang="en">opening hours</rdfs:label>
    </owl:DatatypeProperty>
    


    <!-- http://schema.org/postalCode -->

    <owl:DatatypeProperty rdf:about="http://schema.org/postalCode">
        <rdfs:domain rdf:resource="http://schema.org/PostalAddress"/>
        <rdfs:range rdf:resource="http://www.w3.org/2000/01/rdf-schema#Literal"/>
        <rdfs:comment xml:lang="en">The postal code.</rdfs:comment>
        <rdfs:isDefinedBy rdf:resource="http://schema.org/postalCode"/>
        <rdfs:label xml:lang="fr">code postal</rdfs:label>
        <rdfs:label xml:lang="es">código postal</rdfs:label>
        <rdfs:label xml:lang="en">postal code</rdfs:label>
    </owl:DatatypeProperty>
    


    <!-- http://schema.org/telephone -->

    <owl:DatatypeProperty rdf:about="http://schema.org/telephone">
        <rdfs:domain rdf:resource="http://schema.org/PostalAddress"/>
        <rdfs:range rdf:resource="http://www.w3.org/2000/01/rdf-schema#Literal"/>
        <rdfs:comment xml:lang="en">The telephone number.</rdfs:comment>
        <rdfs:isDefinedBy rdf:resource="http://schema.org/telephone"/>
        <rdfs:label xml:lang="fr">numéro de téléphone</rdfs:label>
        <rdfs:label xml:lang="es">número de teléfono</rdfs:label>
        <rdfs:label xml:lang="en">telephone number</rdfs:label>
    </owl:DatatypeProperty>
    


    <!-- 
    ///////////////////////////////////////////////////////////////////////////////////////
    //
    // Classes
    //
    ///////////////////////////////////////////////////////////////////////////////////////
     -->

    


    <!-- http://lod.ehri-project-test.eu/ontology#AlternateAgentName -->

    <owl:Class rdf:about="http://lod.ehri-project-test.eu/ontology#AlternateAgentName">
        <rdfs:subClassOf rdf:resource="https://www.ica.org/standards/RiC/ontology#AgentName"/>
        <rdfs:comment xml:lang="en">This class allows to represent any other name(s) used for the institution or by which it may be known. This could include other forms of the same name, abbreviations, acronyms, other institutional names, or changes of name over time (historical names).</rdfs:comment>
        <rdfs:label xml:lang="en">Alternative forms of the agent&apos;s name</rdfs:label>
        <rdfs:label xml:lang="es">Formas alternativas del nombre</rdfs:label>
        <rdfs:label xml:lang="fr">Formes alternatives du nom</rdfs:label>
    </owl:Class>
    


    <!-- http://lod.ehri-project-test.eu/ontology#City -->

    <owl:Class rdf:about="http://lod.ehri-project-test.eu/ontology#City">
        <rdfs:subClassOf rdf:resource="https://www.ica.org/standards/RiC/ontology#Place"/>
        <rdfs:comment xml:lang="en">This class represents a city as a more precise type of rico:Place.</rdfs:comment>
        <rdfs:label xml:lang="en">City</rdfs:label>
        <rdfs:label xml:lang="es">Ciudad</rdfs:label>
        <rdfs:label xml:lang="fr">Ville</rdfs:label>
    </owl:Class>
    


    <!-- http://lod.ehri-project-test.eu/ontology#CorporateBody -->

    <owl:Class rdf:about="http://lod.ehri-project-test.eu/ontology#CorporateBody">
        <rdfs:subClassOf rdf:resource="https://www.ica.org/standards/RiC/ontology#CorporateBody"/>
        <rdfs:comment xml:lang="en">This is a specialisation of the rico:CorporateBody class created for its extension with additional properties.</rdfs:comment>
        <rdfs:label xml:lang="fr">Collectivité</rdfs:label>
        <rdfs:label xml:lang="en">Corporate body</rdfs:label>
        <rdfs:label xml:lang="es">Persona jurídica</rdfs:label>
    </owl:Class>
    


    <!-- http://lod.ehri-project-test.eu/ontology#Country -->

    <owl:Class rdf:about="http://lod.ehri-project-test.eu/ontology#Country">
        <rdfs:subClassOf rdf:resource="https://www.ica.org/standards/RiC/ontology#Place"/>
        <rdfs:comment xml:lang="en">This class represents a country as a more precise type of rico:Place.</rdfs:comment>
        <rdfs:label xml:lang="en">Country</rdfs:label>
        <rdfs:label xml:lang="fr">Pays</rdfs:label>
        <rdfs:label xml:lang="es">País</rdfs:label>
    </owl:Class>
    


    <!-- http://lod.ehri-project-test.eu/ontology#Family -->

    <owl:Class rdf:about="http://lod.ehri-project-test.eu/ontology#Family">
        <rdfs:subClassOf rdf:resource="https://www.ica.org/standards/RiC/ontology#Family"/>
        <rdfs:comment xml:lang="en">This is a specialisation of the rico:Family class created for its extension with additional properties.</rdfs:comment>
        <rdfs:label xml:lang="es">Familia</rdfs:label>
        <rdfs:label xml:lang="fr">Famille</rdfs:label>
        <rdfs:label xml:lang="en">Family</rdfs:label>
    </owl:Class>
    


    <!-- http://lod.ehri-project-test.eu/ontology#Institution -->

    <owl:Class rdf:about="http://lod.ehri-project-test.eu/ontology#Institution">
        <rdfs:subClassOf rdf:resource="http://lod.ehri-project-test.eu/ontology#CorporateBody"/>
        <rdfs:subClassOf rdf:resource="http://schema.org/ArchiveOrganization"/>
        <rdfs:comment xml:lang="en">This class is a specialisation of the rico:CorporateBody and ehri:CorporateBody classes, taking some additional properties from the schema:ArchiveOrganization class. By contrast to a Corporate Body, in EHRI&apos;s data model, an Institution always hold archival records which is in line with ISDIAH definition.</rdfs:comment>
        <rdfs:label xml:lang="es">Institución</rdfs:label>
        <rdfs:label xml:lang="en">Institution</rdfs:label>
        <rdfs:label xml:lang="fr">Institution</rdfs:label>
    </owl:Class>
    


    <!-- http://lod.ehri-project-test.eu/ontology#InstitutionAddress -->

    <owl:Class rdf:about="http://lod.ehri-project-test.eu/ontology#InstitutionAddress">
        <rdfs:subClassOf rdf:resource="http://schema.org/PostalAddress"/>
        <rdfs:subClassOf rdf:resource="https://www.ica.org/standards/RiC/ontology#PhysicalLocation"/>
        <rdfs:comment xml:lang="en">This class is a specialisation of the rico:PhysicalLocation extended with attributes coming from the schema:PostalAddress class to represent institution&apos;s addresses and contact information.</rdfs:comment>
        <rdfs:label xml:lang="fr">Adresse de l&apos;institution</rdfs:label>
        <rdfs:label xml:lang="es">Dirección de la institución</rdfs:label>
        <rdfs:label xml:lang="en">Institution&apos;s address</rdfs:label>
    </owl:Class>
    


    <!-- http://lod.ehri-project-test.eu/ontology#MaterialScript -->

    <owl:Class rdf:about="http://lod.ehri-project-test.eu/ontology#MaterialScript">
        <rdfs:subClassOf rdf:resource="https://www.ica.org/standards/RiC/ontology#Concept"/>
        <rdfs:comment xml:lang="en">This class represents the scripts that can be found in a material. Similar to the language, each instance will be represented by an instance. Examples of scripts are: Latin, Cyrillic, etc.</rdfs:comment>
        <rdfs:label xml:lang="es">Escritura de la documentación</rdfs:label>
        <rdfs:label xml:lang="en">Script of materials</rdfs:label>
        <rdfs:label xml:lang="fr">Écriture des documents</rdfs:label>
    </owl:Class>
    


    <!-- http://lod.ehri-project-test.eu/ontology#ParallelAgentName -->

    <owl:Class rdf:about="http://lod.ehri-project-test.eu/ontology#ParallelAgentName">
        <rdfs:subClassOf rdf:resource="https://www.ica.org/standards/RiC/ontology#AgentName"/>
        <rdfs:comment xml:lang="en">This class allows to represent the various forms in which the authorised form of name of an institution with archival holdings occurs in other languages or script form(s).</rdfs:comment>
        <rdfs:label xml:lang="es">Formas paralelas del nombre</rdfs:label>
        <rdfs:label xml:lang="fr">Formes parallèles du nom</rdfs:label>
        <rdfs:label xml:lang="en">Parallel forms of the agent&apos;s name</rdfs:label>
    </owl:Class>
    


    <!-- http://lod.ehri-project-test.eu/ontology#Person -->

    <owl:Class rdf:about="http://lod.ehri-project-test.eu/ontology#Person">
        <rdfs:subClassOf rdf:resource="https://www.ica.org/standards/RiC/ontology#Person"/>
        <rdfs:comment xml:lang="en">This is a specialisation of the rico:Person class created for its extension with additional properties.</rdfs:comment>
        <rdfs:label xml:lang="en">Person</rdfs:label>
        <rdfs:label xml:lang="es">Persona</rdfs:label>
        <rdfs:label xml:lang="fr">Personne</rdfs:label>
    </owl:Class>
    


    <!-- http://lod.ehri-project-test.eu/ontology#Record -->

    <owl:Class rdf:about="http://lod.ehri-project-test.eu/ontology#Record">
        <rdfs:subClassOf rdf:resource="http://lod.ehri-project-test.eu/ontology#RecordResource"/>
        <rdfs:subClassOf rdf:resource="https://www.ica.org/standards/RiC/ontology#Record"/>
        <rdfs:comment xml:lang="en">This is a specialisation of the rico:Record class created for its extension with additional properties.</rdfs:comment>
        <rdfs:label xml:lang="es">Documento</rdfs:label>
        <rdfs:label xml:lang="fr">Objet informationnel</rdfs:label>
        <rdfs:label xml:lang="en">Record</rdfs:label>
    </owl:Class>
    


    <!-- http://lod.ehri-project-test.eu/ontology#RecordResource -->

    <owl:Class rdf:about="http://lod.ehri-project-test.eu/ontology#RecordResource">
        <rdfs:subClassOf rdf:resource="https://www.ica.org/standards/RiC/ontology#RecordResource"/>
        <rdfs:comment xml:lang="en">This is a specialisation of the rico:RecordResource class created for its extension with additional properties.</rdfs:comment>
        <rdfs:label xml:lang="en">Record Resource</rdfs:label>
        <rdfs:label xml:lang="es">Recurso documental</rdfs:label>
        <rdfs:label xml:lang="fr">Ressource archivistique</rdfs:label>
    </owl:Class>
    


    <!-- http://lod.ehri-project-test.eu/ontology#RecordSet -->

    <owl:Class rdf:about="http://lod.ehri-project-test.eu/ontology#RecordSet">
        <rdfs:subClassOf rdf:resource="http://lod.ehri-project-test.eu/ontology#RecordResource"/>
        <rdfs:subClassOf rdf:resource="https://www.ica.org/standards/RiC/ontology#RecordSet"/>
        <rdfs:comment xml:lang="en">This is a specialisation of the rico:RecordSet class created for its extension with additional properties.</rdfs:comment>
        <rdfs:label xml:lang="es">Agrupación documental</rdfs:label>
        <rdfs:label xml:lang="fr">Ensemble d’objets informationnels</rdfs:label>
        <rdfs:label xml:lang="en">Record set</rdfs:label>
    </owl:Class>
    


    <!-- http://lod.ehri-project-test.eu/ontology#Region -->

    <owl:Class rdf:about="http://lod.ehri-project-test.eu/ontology#Region">
        <rdfs:subClassOf rdf:resource="https://www.ica.org/standards/RiC/ontology#Place"/>
        <rdfs:comment xml:lang="en">This class represents a region as a more precise type of rico:Place.</rdfs:comment>
        <rdfs:label xml:lang="en">Region</rdfs:label>
        <rdfs:label xml:lang="es">Región</rdfs:label>
        <rdfs:label xml:lang="fr">Région</rdfs:label>
    </owl:Class>
    


    <!-- http://schema.org/ArchiveOrganization -->

    <owl:Class rdf:about="http://schema.org/ArchiveOrganization"/>
    


    <!-- http://schema.org/PostalAddress -->

    <owl:Class rdf:about="http://schema.org/PostalAddress"/>
    


    <!-- http://www.w3.org/2004/02/skos/core#Concept -->

    <rdf:Description rdf:about="http://www.w3.org/2004/02/skos/core#Concept">
        <rdfs:subClassOf rdf:resource="https://www.ica.org/standards/RiC/ontology#Thing"/>
    </rdf:Description>
    


    <!-- 
    ///////////////////////////////////////////////////////////////////////////////////////
    //
    // Individuals
    //
    ///////////////////////////////////////////////////////////////////////////////////////
     -->

    


    <!-- http://lod.ehri-project-test.eu/vocabularies/recordSetTypes#RecordGroup -->

    <owl:NamedIndividual rdf:about="http://lod.ehri-project-test.eu/vocabularies/recordSetTypes#RecordGroup">
        <rdf:type rdf:resource="http://www.w3.org/2004/02/skos/core#Concept"/>
        <rdf:type rdf:resource="https://www.ica.org/standards/RiC/ontology#RecordSetType"/>
        <skos:inScheme rdf:resource="https://www.ica.org/standards/RiC/vocabularies/recordSetTypes"/>
        <skos:topConceptOf rdf:resource="https://www.ica.org/standards/RiC/vocabularies/recordSetTypes"/>
        <rdfs:label xml:lang="fr">groupe d&apos;enregistrement</rdfs:label>
        <rdfs:label xml:lang="en">record group</rdfs:label>
        <rdfs:label xml:lang="es">unidad documental compuesta</rdfs:label>
    </owl:NamedIndividual>
    


    <!-- http://lod.ehri-project-test.eu/vocabularies/recordSetTypes#Subcollection -->

    <owl:NamedIndividual rdf:about="http://lod.ehri-project-test.eu/vocabularies/recordSetTypes#Subcollection">
        <rdf:type rdf:resource="http://www.w3.org/2004/02/skos/core#Concept"/>
        <rdf:type rdf:resource="https://www.ica.org/standards/RiC/ontology#RecordSetType"/>
        <skos:inScheme rdf:resource="https://www.ica.org/standards/RiC/vocabularies/recordSetTypes"/>
        <skos:topConceptOf rdf:resource="https://www.ica.org/standards/RiC/vocabularies/recordSetTypes"/>
        <rdfs:label xml:lang="fr">sous-collection</rdfs:label>
        <rdfs:label xml:lang="en">sub-collection</rdfs:label>
        <rdfs:label xml:lang="es">subcolección</rdfs:label>
    </owl:NamedIndividual>
    


    <!-- http://lod.ehri-project-test.eu/vocabularies/recordSetTypes#Subfonds -->

    <owl:NamedIndividual rdf:about="http://lod.ehri-project-test.eu/vocabularies/recordSetTypes#Subfonds">
        <rdf:type rdf:resource="http://www.w3.org/2004/02/skos/core#Concept"/>
        <rdf:type rdf:resource="https://www.ica.org/standards/RiC/ontology#RecordSetType"/>
        <skos:inScheme rdf:resource="https://www.ica.org/standards/RiC/vocabularies/recordSetTypes"/>
        <skos:topConceptOf rdf:resource="https://www.ica.org/standards/RiC/vocabularies/recordSetTypes"/>
        <rdfs:label xml:lang="fr">sous-fonds</rdfs:label>
        <rdfs:label xml:lang="en">sub-fonds</rdfs:label>
        <rdfs:label xml:lang="es">subfondo</rdfs:label>
    </owl:NamedIndividual>
    


    <!-- http://lod.ehri-project-test.eu/vocabularies/recordSetTypes#Subgroup -->

    <owl:NamedIndividual rdf:about="http://lod.ehri-project-test.eu/vocabularies/recordSetTypes#Subgroup">
        <rdf:type rdf:resource="http://www.w3.org/2004/02/skos/core#Concept"/>
        <rdf:type rdf:resource="https://www.ica.org/standards/RiC/ontology#RecordSetType"/>
        <skos:inScheme rdf:resource="https://www.ica.org/standards/RiC/vocabularies/recordSetTypes"/>
        <skos:topConceptOf rdf:resource="https://www.ica.org/standards/RiC/vocabularies/recordSetTypes"/>
        <rdfs:label xml:lang="fr">sous-groupe</rdfs:label>
        <rdfs:label xml:lang="en">sub-group</rdfs:label>
        <rdfs:label xml:lang="es">subunidad documental compuesta</rdfs:label>
    </owl:NamedIndividual>
    


    <!-- http://lod.ehri-project-test.eu/vocabularies/recordSetTypes#Subseries -->

    <owl:NamedIndividual rdf:about="http://lod.ehri-project-test.eu/vocabularies/recordSetTypes#Subseries">
        <rdf:type rdf:resource="http://www.w3.org/2004/02/skos/core#Concept"/>
        <rdf:type rdf:resource="https://www.ica.org/standards/RiC/ontology#RecordSetType"/>
        <skos:inScheme rdf:resource="https://www.ica.org/standards/RiC/vocabularies/recordSetTypes"/>
        <skos:topConceptOf rdf:resource="https://www.ica.org/standards/RiC/vocabularies/recordSetTypes"/>
        <rdfs:label xml:lang="fr">sous-série</rdfs:label>
        <rdfs:label xml:lang="en">sub-series</rdfs:label>
        <rdfs:label xml:lang="es">subserie</rdfs:label>
    </owl:NamedIndividual>
</rdf:RDF>



<!-- Generated by the OWL API (version 4.5.29.2024-05-13T12:11:03Z) https://github.com/owlcs/owlapi -->
