@prefix : <http://lod.ehri-project-test.eu/ontology#> .
@prefix owl: <http://www.w3.org/2002/07/owl#> .
@prefix rdf: <http://www.w3.org/1999/02/22-rdf-syntax-ns#> .
@prefix xml: <http://www.w3.org/XML/1998/namespace> .
@prefix xsd: <http://www.w3.org/2001/XMLSchema#> .
@prefix rdfs: <http://www.w3.org/2000/01/rdf-schema#> .
@base <http://lod.ehri-project-test.eu/ontology#> .

<http://lod.ehri-project-test.eu/ontology> rdf:type owl:Ontology ;
                                            owl:versionIRI <http://lod.ehri-project-test.eu/ontology/0.0.3> ;
                                            owl:imports <https://www.ica.org/standards/RiC/ontology/1.0.2> ;
                                            <http://creativecommons.org/ns#license> <https://creativecommons.org/licenses/by/4.0/> ;
                                            <http://purl.org/dc/elements/1.1/creator> "Herminio García-González (Kazerne Dossin)"@en ,
                                                                                      "Mike Bryant (NIOD)"@en ;
                                            <http://purl.org/dc/elements/1.1/title> "EHRI Ontology"@en ;
                                            <http://purl.org/dc/terms/abstract> "This ontology defines the data model used by the EHRI Knowledge Graph for the representation of the information hosted in the EHRI Portal. It does so by extending RiC-O v1.0.2 and reusing some of the schema.org concepts."@en ;
                                            <http://purl.org/dc/terms/description> "The EHRI Ontology extends some of the RiC-O types and adds additional properties to represent data present in the EHRI Portal. Whenever a class is extended with new properties, a subclass bounded to the ehri prefix is created in order to maintain the original RiC-O axioms. In some cases, classes are specialised via subclassing in order to contribute additional meaning to the superclass."@en ;
                                            <http://purl.org/dc/terms/publisher> "EHRI-ERIC" ;
                                            <http://purl.org/vocab/vann/preferredNamespacePrefix> "ehri" ;
                                            <http://purl.org/vocab/vann/preferredNamespaceUri> : ;
                                            <http://schema.org/codeRepository> <https://github.com/EHRI/ehri-kg-ontology> ;
                                            <http://schema.org/funder> <https://oscars-project.eu/> ;
                                            <http://schema.org/funding> <https://oscars-project.eu/projects/ehri-kg-european-holocaust-research-infrastructure-knowledge-graph> ;
                                            owl:priorVersion <http://lod.ehri-project-test.eu/ontology/0.0.2> ;
                                            owl:versionInfo "0.0.3" ;
                                            <http://xmlns.com/foaf/0.1/logo> <https://ehri-kg.ehri-project.eu/images/ehri-logo.svg> .

#################################################################
#    Annotation properties
#################################################################

###  http://purl.org/dc/elements/1.1/contributor
<http://purl.org/dc/elements/1.1/contributor> rdf:type owl:AnnotationProperty ;
                                              rdfs:subPropertyOf rdfs:comment .


###  http://purl.org/vocab/vann/preferredNamespacePrefix
<http://purl.org/vocab/vann/preferredNamespacePrefix> rdf:type owl:AnnotationProperty .


###  http://purl.org/vocab/vann/preferredNamespaceUri
<http://purl.org/vocab/vann/preferredNamespaceUri> rdf:type owl:AnnotationProperty .


###  http://schema.org/codeRepository
<http://schema.org/codeRepository> rdf:type owl:AnnotationProperty .


###  http://schema.org/funder
<http://schema.org/funder> rdf:type owl:AnnotationProperty .


###  http://schema.org/funding
<http://schema.org/funding> rdf:type owl:AnnotationProperty .


###  http://www.w3.org/2004/02/skos/core#definition
<http://www.w3.org/2004/02/skos/core#definition> rdf:type owl:AnnotationProperty .


###  http://xmlns.com/foaf/0.1/logo
<http://xmlns.com/foaf/0.1/logo> rdf:type owl:AnnotationProperty .


#################################################################
#    Object Properties
#################################################################

###  http://lod.ehri-project-test.eu/ontology#hasCopy
:hasCopy rdf:type owl:ObjectProperty ;
         rdfs:subPropertyOf <https://www.ica.org/standards/RiC/ontology#hasCopy> ,
                            <https://www.ica.org/standards/RiC/ontology#isRelatedTo> ;
         owl:inverseOf :isCopyOf ;
         rdfs:domain [ rdf:type owl:Class ;
                       owl:unionOf ( :Institution
                                     :RecordResource
                                   )
                     ] ;
         rdfs:range [ rdf:type owl:Class ;
                      owl:unionOf ( :Institution
                                    :RecordResource
                                  )
                    ] ;
         rdfs:comment "A generalisation of the rico:hasCopy property to expand the domain and range to ehri:Institution instances."@en ;
         rdfs:label "a pour copie"@fr ,
                    "has copy"@en ,
                    "tiene como copia"@es .


###  http://lod.ehri-project-test.eu/ontology#hasOrHadScript
:hasOrHadScript rdf:type owl:ObjectProperty ;
                rdfs:subPropertyOf <https://www.ica.org/standards/RiC/ontology#isRelatedTo> ;
                owl:inverseOf :isOrWasScriptOf ;
                rdfs:domain :RecordResource ;
                rdfs:range :MaterialScript ;
                rdfs:comment "Indicates the written script present in the materials."@en ;
                rdfs:label "a ou a eu pour écriture"@fr ,
                           "has or had script"@en ,
                           "tiene o tenía como escritura"@es .


###  http://lod.ehri-project-test.eu/ontology#isCopyOf
:isCopyOf rdf:type owl:ObjectProperty ;
          rdfs:subPropertyOf <https://www.ica.org/standards/RiC/ontology#isCopyOf> ,
                             <https://www.ica.org/standards/RiC/ontology#isRelatedTo> ;
          rdfs:domain [ rdf:type owl:Class ;
                        owl:unionOf ( :Institution
                                      :RecordResource
                                    )
                      ] ;
          rdfs:range [ rdf:type owl:Class ;
                       owl:unionOf ( :Institution
                                     :RecordResource
                                   )
                     ] ;
          rdfs:comment "Inverse of ehri:hasCopy object property."@en ;
          rdfs:label "es copia de"@es ,
                     "est la copie de"@fr ,
                     "is copy of"@en .


###  http://lod.ehri-project-test.eu/ontology#isOrWasScriptOf
:isOrWasScriptOf rdf:type owl:ObjectProperty ;
                 rdfs:subPropertyOf <https://www.ica.org/standards/RiC/ontology#isRelatedTo> ;
                 rdfs:domain :MaterialScript ;
                 rdfs:range :RecordResource ;
                 rdfs:comment "The inverse of ehri:hasOrHadScript, allowing a script to be related back to the record where it appears."@en ;
                 rdfs:label "es o era la escritura de"@es ,
                            "est ou était l'ecriture de"@fr ,
                            "is or was the script of"@en .


#################################################################
#    Data properties
#################################################################

###  http://lod.ehri-project-test.eu/ontology#accessibility
:accessibility rdf:type owl:DatatypeProperty ;
               rdfs:domain :Institution ;
               rdfs:range rdfs:Literal ;
               rdfs:comment "Collects information about the accessibility of an institution with respect to its archival holdings and services."@en ;
               rdfs:label "accesibilidad"@es ,
                          "accessibility"@en ,
                          "accessibilité"@fr .


###  http://lod.ehri-project-test.eu/ontology#administrativeStructure
:administrativeStructure rdf:type owl:DatatypeProperty ;
                         rdfs:domain :Institution ;
                         rdfs:range rdfs:Literal ;
                         rdfs:comment "Represents the current administrative structure of an institution."@en ;
                         rdfs:label "administrative structure"@en ,
                                    "estructura administrativa"@es ,
                                    "structure administrative"@fr .


###  http://lod.ehri-project-test.eu/ontology#appraisal
:appraisal rdf:type owl:DatatypeProperty ;
           rdfs:domain :RecordResource ;
           rdfs:range rdfs:Literal ;
           rdfs:comment "Provides information on appraisal, destruction and scheduling actions."@en ;
           rdfs:label "appraisal"@en ,
                      "valoración"@es ,
                      "évaluation"@fr .


###  http://lod.ehri-project-test.eu/ontology#archivalHistory
:archivalHistory rdf:type owl:DatatypeProperty ;
                 rdfs:subPropertyOf <https://www.ica.org/standards/RiC/ontology#history> ;
                 rdfs:domain :Country ;
                 rdfs:range rdfs:Literal ;
                 rdfs:comment "Provides information about the Holocaust and WWII and how it relates to the archival landscape in that country."@en ;
                 rdfs:label "archival history"@en ,
                            "histoire archivistique"@fr ,
                            "historia archivística"@es .


###  http://lod.ehri-project-test.eu/ontology#archivalSituation
:archivalSituation rdf:type owl:DatatypeProperty ;
                   rdfs:domain :Country ;
                   rdfs:range rdfs:Literal ;
                   rdfs:comment "Offers a short introduction to the archival situation and culture in a country."@en ;
                   rdfs:label "archival situation"@en ,
                              "situación de los archivos"@es ,
                              "situation de conservation"@fr .


###  http://lod.ehri-project-test.eu/ontology#archivistNote
:archivistNote rdf:type owl:DatatypeProperty ;
               rdfs:subPropertyOf :notes ;
               rdfs:domain :RecordResource ;
               rdfs:range rdfs:Literal ;
               rdfs:comment "Explains how the description was prepared and by whom."@en ;
               rdfs:label "archivist note"@en ,
                          "nota del archivero/a"@es ,
                          "notes de l'archiviste"@fr .


###  http://lod.ehri-project-test.eu/ontology#buildings
:buildings rdf:type owl:DatatypeProperty ;
           rdfs:domain :Institution ;
           rdfs:range rdfs:Literal ;
           rdfs:comment "Provides information about the buildings of an institution."@en ;
           rdfs:label "building(s)"@en ,
                      "bâtiment(s)"@fr ,
                      "edificio(s)"@es .


###  http://lod.ehri-project-test.eu/ontology#conditionsOfAccess
:conditionsOfAccess rdf:type owl:DatatypeProperty ;
                    rdfs:subPropertyOf <https://www.ica.org/standards/RiC/ontology#conditionsOfAccess> ;
                    rdfs:domain [ rdf:type owl:Class ;
                                  owl:unionOf ( :Institution
                                                :RecordResource
                                              )
                                ] ;
                    rdfs:range rdfs:Literal ;
                    rdfs:comment "Collects information about the conditions, requirements and procedures for access to, and use of institutional services and/or specific records."@en ;
                    rdfs:label "condiciones de acceso"@es ,
                               "conditions d'accès"@fr ,
                               "conditions of access"@en .


###  http://lod.ehri-project-test.eu/ontology#contactPerson
:contactPerson rdf:type owl:DatatypeProperty ;
               rdfs:domain :InstitutionAddress ;
               rdfs:range rdfs:Literal ;
               rdfs:comment "Provides information needed to contact members of the staff."@en ;
               rdfs:label "contact person"@en ,
                          "persona de contacto"@es ,
                          "personne de contact"@fr .


###  http://lod.ehri-project-test.eu/ontology#findingAids
:findingAids rdf:type owl:DatatypeProperty ;
             rdfs:domain :Institution ;
             rdfs:range rdfs:Literal ;
             rdfs:comment "Provides a general overview of finding aids published by an institution."@en ;
             rdfs:label "finding aids"@en ,
                        "instrumentos de descripción"@es ,
                        "instruments de recherche"@fr .


###  http://lod.ehri-project-test.eu/ontology#generalContext
:generalContext rdf:type owl:DatatypeProperty ;
                rdfs:subPropertyOf <https://www.ica.org/standards/RiC/ontology#generalDescription> ;
                rdfs:domain :Institution ;
                rdfs:range rdfs:Literal ;
                rdfs:comment "Provides information about the geographical and cultural context of an institution."@en ;
                rdfs:label "contexte général"@fr ,
                           "contexto general"@es ,
                           "general context"@en .


###  http://lod.ehri-project-test.eu/ontology#locationOfCopies
:locationOfCopies rdf:type owl:DatatypeProperty ;
                  rdfs:domain :RecordResource ;
                  rdfs:range rdfs:Literal ;
                  rdfs:comment "Indicates the existence, location and availability of copies of the unit of description."@en ;
                  rdfs:label "existence and location of copies"@en ,
                             "existence et lieu de copies"@fr ,
                             "existencia y localización de copias"@es .


###  http://lod.ehri-project-test.eu/ontology#locationOfOriginals
:locationOfOriginals rdf:type owl:DatatypeProperty ;
                     rdfs:domain :RecordResource ;
                     rdfs:range rdfs:Literal ;
                     rdfs:comment "Indicates the existence, location, availability and/or destruction of the original material, in cases where the unit of description consists of copies."@en ;
                     rdfs:label "existence and location of originals"@en ,
                                "existence et lieu des originaux"@fr ,
                                "existencia y localización de los originales"@es .


###  http://lod.ehri-project-test.eu/ontology#notes
:notes rdf:type owl:DatatypeProperty ;
       rdfs:domain :RecordResource ;
       rdfs:range rdfs:Literal ;
       rdfs:comment "Provides information that cannot be accommodated in any of the other data properties."@en ;
       rdfs:label "nota(s)"@es ,
                  "note(s)"@en ,
                  "note(s)"@fr .


###  http://lod.ehri-project-test.eu/ontology#otherFindingAids
:otherFindingAids rdf:type owl:DatatypeProperty ;
                  rdfs:domain :RecordResource ;
                  rdfs:range rdfs:Literal ;
                  rdfs:comment "Provides information on the history of the unit of description that is significant for its authenticity, integrity and interpretation."@en ;
                  rdfs:label "autres instruments de recherche"@fr ,
                             "other finding aids"@en ,
                             "otros instrumentos de descripción"@es .


###  http://lod.ehri-project-test.eu/ontology#physicalCharacterisiticsAndTechnicalRequirements
:physicalCharacterisiticsAndTechnicalRequirements rdf:type owl:DatatypeProperty ;
                                                  rdfs:domain :RecordResource ;
                                                  rdfs:range rdfs:Literal ;
                                                  rdfs:comment "Collects information about any important physical characteristics or technical requirements that affect use of the unit of description."@en ;
                                                  rdfs:label "características físicas y requisitos técnicos"@es ,
                                                             "caractéristiques matérielles et contraintes techniques"@fr ,
                                                             "physical characteristics and technical requirements"@en .


###  http://lod.ehri-project-test.eu/ontology#publicAreas
:publicAreas rdf:type owl:DatatypeProperty ;
             rdfs:domain :Institution ;
             rdfs:range rdfs:Literal ;
             rdfs:comment "Collects information about areas of the institution available for public use."@en ;
             rdfs:label "espaces publics"@fr ,
                        "espacios públicos"@es ,
                        "public areas"@en .


###  http://lod.ehri-project-test.eu/ontology#publicationNote
:publicationNote rdf:type owl:DatatypeProperty ;
                 rdfs:domain :RecordResource ;
                 rdfs:range rdfs:Literal ;
                 rdfs:comment "Identifies any publications that are about or are based on the use, study or analysis of the unit of description."@en ;
                 rdfs:label "bibliographie"@fr ,
                            "nota de publicaciones"@es ,
                            "publication note"@en .


###  http://lod.ehri-project-test.eu/ontology#recordsManagementAndCollectingPolicies
:recordsManagementAndCollectingPolicies rdf:type owl:DatatypeProperty ;
                                        rdfs:domain :Institution ;
                                        rdfs:range rdfs:Literal ;
                                        rdfs:comment "Provides information about the records management and collecting policies of an institution with archival holdings."@en ;
                                        rdfs:label "gestion des archives courantes et intermédiaires et politiques de collecte"@fr ,
                                                   "gestión de documentos y política de ingresos"@es ,
                                                   "records management and collecting policies"@en .


###  http://lod.ehri-project-test.eu/ontology#relatedMaterial
:relatedMaterial rdf:type owl:DatatypeProperty ;
                 rdfs:domain :RecordResource ;
                 rdfs:range rdfs:Literal ;
                 rdfs:comment "Identifies related units of description."@en ;
                 rdfs:label "related units of description"@en ,
                            "sources complémentaires"@fr ,
                            "unidades de descripción relacionadas"@es .


###  http://lod.ehri-project-test.eu/ontology#reproductionServices
:reproductionServices rdf:type owl:DatatypeProperty ;
                      rdfs:domain :Institution ;
                      rdfs:range rdfs:Literal ;
                      rdfs:comment "Provides information about reproduction services available to the public (microfilms, photocopies, photographs, digitised copies) and their general conditions and restrictions."@en ;
                      rdfs:label "reproduction services"@en ,
                                 "services de reproduction"@fr ,
                                 "servicios de reproducción"@es .


###  http://lod.ehri-project-test.eu/ontology#researchExtensive
:researchExtensive rdf:type owl:DatatypeProperty ;
                   rdfs:domain :Country ;
                   rdfs:range rdfs:Literal ;
                   rdfs:comment "Offers information on how EHRI acquired data relating to a country and integrated it into the EHRI Portal."@en ;
                   rdfs:label "investigación del EHRI (ampliado)"@es ,
                              "recherche par EHRI (extensif)"@fr ,
                              "research by EHRI (extensive)"@en .


###  http://lod.ehri-project-test.eu/ontology#researchServices
:researchServices rdf:type owl:DatatypeProperty ;
                  rdfs:domain :Institution ;
                  rdfs:range rdfs:Literal ;
                  rdfs:comment "Describes the research services provided by an institution."@en ;
                  rdfs:label "research services"@en ,
                             "services d'aide à la recherche"@fr ,
                             "servicios de ayuda a la investigación"@es .


###  http://lod.ehri-project-test.eu/ontology#researchSummary
:researchSummary rdf:type owl:DatatypeProperty ;
                 rdfs:domain :Country ;
                 rdfs:range rdfs:Literal ;
                 rdfs:comment "Describes the identification work carried out by EHRI, ongoing since October 2010. This section also includes references to aggregators and country-specific research guides."@en ;
                 rdfs:label "investigación del EHRI (resumen)"@es ,
                            "recherche EHRI (récapitulatif)"@fr ,
                            "research by EHRI (summary)"@en .


###  http://lod.ehri-project-test.eu/ontology#separatedMaterial
:separatedMaterial rdf:type owl:DatatypeProperty ;
                   rdfs:domain :RecordResource ;
                   rdfs:range rdfs:Literal ;
                   rdfs:comment "Information about materials that are associated by provenance to the described materials but that have been physically separated or removed. Items may be separated for various reasons, including the dispersal of special formats to more appropriate custodial units; the outright destruction of duplicate or nonessential material; and the deliberate or unintentional scattering of fonds among different repositories."@en ;
                   rdfs:label "separated units of description"@en ,
                              "sources séparées"@fr ,
                              "unidadades de descripción separadas"@es .


###  http://lod.ehri-project-test.eu/ontology#sources
:sources rdf:type owl:DatatypeProperty ;
         rdfs:domain [ rdf:type owl:Class ;
                       owl:unionOf ( :Agent
                                     :RecordResource
                                   )
                     ] ;
         rdfs:range rdfs:Literal ;
         rdfs:comment "Provides information on sources consulted in preparing the description and the personnel involved."@en ;
         rdfs:label "fuentes"@es ,
                    "sources"@en ,
                    "sources"@fr .


###  http://lod.ehri-project-test.eu/ontology#structureOrGenealogy
:structureOrGenealogy rdf:type owl:DatatypeProperty ;
                      rdfs:domain :Agent ;
                      rdfs:range rdfs:Literal ;
                      rdfs:comment "Describes and/or represents the internal administrative structure(s) of a corporate body or the genealogy of a family."@en ;
                      rdfs:label "estructura(s) interna(s)/genealogía"@es ,
                                 "internal structure"@en ,
                                 "structure interne"@fr .


###  http://schema.org/contactType
<http://schema.org/contactType> rdf:type owl:DatatypeProperty ;
                                rdfs:domain <http://schema.org/PostalAddress> ;
                                rdfs:range rdfs:Literal ;
                                rdfs:comment "Specifies the type of contact point. A person or organization can have different contact points for different purposes, such as a sales contact point, a PR contact point and so on."@en ;
                                rdfs:isDefinedBy <http://schema.org/contactType> ;
                                rdfs:label "contact type"@en ,
                                           "tipo de contacto"@es ,
                                           "type de contact"@fr .


###  http://schema.org/email
<http://schema.org/email> rdf:type owl:DatatypeProperty ;
                          rdfs:domain <http://schema.org/PostalAddress> ;
                          rdfs:range rdfs:Literal ;
                          rdfs:comment "Email address."@en ;
                          rdfs:isDefinedBy <http://schema.org/email> ;
                          rdfs:label "adresse email"@fr ,
                                     "dirección de correo electrónico"@es ,
                                     "email address"@en .


###  http://schema.org/faxNumber
<http://schema.org/faxNumber> rdf:type owl:DatatypeProperty ;
                              rdfs:domain <http://schema.org/PostalAddress> ;
                              rdfs:range rdfs:Literal ;
                              rdfs:comment "The fax number."@en ;
                              rdfs:isDefinedBy <http://schema.org/faxNumber> ;
                              rdfs:label "fax number"@en ,
                                         "numéro de fax"@fr ,
                                         "número de fax"@es .


###  http://schema.org/openingHours
<http://schema.org/openingHours> rdf:type owl:DatatypeProperty ;
                                 rdfs:domain <http://schema.org/ArchiveOrganization> ;
                                 rdfs:range rdfs:Literal ;
                                 rdfs:comment "The general opening hours for a business."@en ;
                                 rdfs:label <http://schema.org/openingHours> ,
                                            "heures d'ouverture"@fr ,
                                            "horarios de apertura"@es ,
                                            "opening hours"@en .


###  http://schema.org/postalCode
<http://schema.org/postalCode> rdf:type owl:DatatypeProperty ;
                               rdfs:domain <http://schema.org/PostalAddress> ;
                               rdfs:range rdfs:Literal ;
                               rdfs:comment "The postal code."@en ;
                               rdfs:isDefinedBy <http://schema.org/postalCode> ;
                               rdfs:label "code postal"@fr ,
                                          "código postal"@es ,
                                          "postal code"@en .


###  http://schema.org/telephone
<http://schema.org/telephone> rdf:type owl:DatatypeProperty ;
                              rdfs:domain <http://schema.org/PostalAddress> ;
                              rdfs:range rdfs:Literal ;
                              rdfs:comment "The telephone number."@en ;
                              rdfs:isDefinedBy <http://schema.org/telephone> ;
                              rdfs:label "numéro de téléphone"@fr ,
                                         "número de teléfono"@es ,
                                         "telephone number"@en .


#################################################################
#    Classes
#################################################################

###  http://lod.ehri-project-test.eu/ontology#Agent
:Agent rdf:type owl:Class ;
       rdfs:subClassOf <https://www.ica.org/standards/RiC/ontology#Agent> ;
       rdfs:comment "This is a specialisation of the rico:Agent class created for its extension with additional properties."@en ;
       rdfs:label "Agent"@en ,
                  "Agent"@fr ,
                  "Agente"@es .


###  http://lod.ehri-project-test.eu/ontology#AlternateAgentName
:AlternateAgentName rdf:type owl:Class ;
                    rdfs:subClassOf <https://www.ica.org/standards/RiC/ontology#AgentName> ;
                    rdfs:comment "This class allows to represent any other name(s) used for an institution, or by which it may be known. This could include other forms of the same name, abbreviations, acronyms, other institutional names, or changes of name over time (historical names)."@en ;
                    rdfs:label "Alternative forms of the agent's name"@en ,
                               "Formas alternativas del nombre"@es ,
                               "Formes alternatives du nom"@fr .


###  http://lod.ehri-project-test.eu/ontology#City
:City rdf:type owl:Class ;
      rdfs:subClassOf <https://www.ica.org/standards/RiC/ontology#Place> ;
      rdfs:comment "This class represents a city as a more precise type of rico:Place."@en ;
      rdfs:label "City"@en ,
                 "Ciudad"@es ,
                 "Ville"@fr .


###  http://lod.ehri-project-test.eu/ontology#CorporateBody
:CorporateBody rdf:type owl:Class ;
               rdfs:subClassOf :Group ,
                               <https://www.ica.org/standards/RiC/ontology#CorporateBody> ;
               rdfs:comment "This is a specialisation of the rico:CorporateBody class created for its extension with additional properties."@en ;
               rdfs:label "Collectivité"@fr ,
                          "Corporate body"@en ,
                          "Persona jurídica"@es .


###  http://lod.ehri-project-test.eu/ontology#Country
:Country rdf:type owl:Class ;
         rdfs:subClassOf <https://www.ica.org/standards/RiC/ontology#Place> ;
         rdfs:comment "This class represents a country as a more precise type of rico:Place."@en ;
         rdfs:label "Country"@en ,
                    "Pays"@fr ,
                    "País"@es .


###  http://lod.ehri-project-test.eu/ontology#Family
:Family rdf:type owl:Class ;
        rdfs:subClassOf :Group ,
                        <https://www.ica.org/standards/RiC/ontology#Family> ;
        rdfs:comment "This is a specialisation of the rico:Family class created for its extension with additional properties."@en ;
        rdfs:label "Familia"@es ,
                   "Famille"@fr ,
                   "Family"@en .


###  http://lod.ehri-project-test.eu/ontology#Group
:Group rdf:type owl:Class ;
       rdfs:subClassOf :Agent ,
                       <https://www.ica.org/standards/RiC/ontology#Group> ;
       rdfs:comment "This is a specialisation of the rico:Group class created for its extension with additional properties."@en ;
       rdfs:label "Group"@en ,
                  "Groupe d'agents"@fr ,
                  "Grupo de agentes"@es .


###  http://lod.ehri-project-test.eu/ontology#Institution
:Institution rdf:type owl:Class ;
             rdfs:subClassOf :CorporateBody ,
                             <http://schema.org/ArchiveOrganization> ;
             rdfs:comment "This class is a specialisation of the rico:CorporateBody and ehri:CorporateBody classes, taking some additional properties from the schema:ArchiveOrganization class. In contrast to a Corporate Body, an Institution in the EHRI data model always holds archival records, which is in line with ISDIAH definition."@en ;
             rdfs:label "Institución"@es ,
                        "Institution"@en ,
                        "Institution"@fr .


###  http://lod.ehri-project-test.eu/ontology#InstitutionAddress
:InstitutionAddress rdf:type owl:Class ;
                    rdfs:subClassOf <http://schema.org/PostalAddress> ,
                                    <https://www.ica.org/standards/RiC/ontology#PhysicalLocation> ;
                    rdfs:comment "This class is a specialisation of the rico:PhysicalLocation extended with attributes derived from the schema:PostalAddress class to represent addresses and contact information for archival institutions."@en ;
                    rdfs:label "Adresse de l'institution"@fr ,
                               "Dirección de la institución"@es ,
                               "Institution's address"@en .


###  http://lod.ehri-project-test.eu/ontology#MaterialScript
:MaterialScript rdf:type owl:Class ;
                rdfs:subClassOf <https://www.ica.org/standards/RiC/ontology#Concept> ;
                rdfs:comment "This class represents the written scripts that can be found in some material. Similar to the written language, each will be represented by an instance. Examples of scripts are: Latin, Cyrillic, Hebrew, etc."@en ;
                rdfs:label "Escritura de la documentación"@es ,
                           "Script of materials"@en ,
                           "Écriture des documents"@fr .


###  http://lod.ehri-project-test.eu/ontology#ParallelAgentName
:ParallelAgentName rdf:type owl:Class ;
                   rdfs:subClassOf <https://www.ica.org/standards/RiC/ontology#AgentName> ;
                   rdfs:comment "This class represents the various forms in which the authorised form of name of an institution with archival holdings occurs in other languages or script form(s)."@en ;
                   rdfs:label "Formas paralelas del nombre"@es ,
                              "Formes parallèles du nom"@fr ,
                              "Parallel forms of the agent's name"@en .


###  http://lod.ehri-project-test.eu/ontology#Person
:Person rdf:type owl:Class ;
        rdfs:subClassOf :Agent ,
                        <https://www.ica.org/standards/RiC/ontology#Person> ;
        rdfs:comment "This is a specialisation of the rico:Person class created for its extension with additional properties."@en ;
        rdfs:label "Person"@en ,
                   "Persona"@es ,
                   "Personne"@fr .


###  http://lod.ehri-project-test.eu/ontology#RecordResource
:RecordResource rdf:type owl:Class ;
                rdfs:subClassOf <https://www.ica.org/standards/RiC/ontology#RecordResource> ;
                rdfs:comment "This is a specialisation of the rico:RecordResource class created for its extension with additional properties."@en ;
                rdfs:label "Record resource"@en ,
                           "Recurso documental"@es ,
                           "Ressource archivistique"@fr .


###  http://lod.ehri-project-test.eu/ontology#RecordSet
:RecordSet rdf:type owl:Class ;
           rdfs:subClassOf :RecordResource ,
                           <https://www.ica.org/standards/RiC/ontology#RecordSet> ;
           rdfs:comment "This is a specialisation of the rico:RecordSet class created for its extension with additional properties."@en ;
           rdfs:label "Agrupación documental"@es ,
                      "Ensemble d’objets informationnels"@fr ,
                      "Record set"@en .


###  http://lod.ehri-project-test.eu/ontology#Region
:Region rdf:type owl:Class ;
        rdfs:subClassOf <https://www.ica.org/standards/RiC/ontology#Place> ;
        rdfs:comment "This class represents a region as a more precise type of rico:Place."@en ;
        rdfs:label "Region"@en ,
                   "Región"@es ,
                   "Région"@fr .


###  http://schema.org/ArchiveOrganization
<http://schema.org/ArchiveOrganization> rdf:type owl:Class .


###  http://schema.org/PostalAddress
<http://schema.org/PostalAddress> rdf:type owl:Class .


###  http://www.w3.org/2004/02/skos/core#Concept
<http://www.w3.org/2004/02/skos/core#Concept> rdfs:subClassOf <https://www.ica.org/standards/RiC/ontology#Thing> .


#################################################################
#    Individuals
#################################################################

###  http://lod.ehri-project-test.eu/ontology#Item
:Item rdf:type owl:NamedIndividual ,
               <http://www.w3.org/2004/02/skos/core#Concept> ,
               <https://www.ica.org/standards/RiC/ontology#RecordSetType> ;
      <http://www.w3.org/2004/02/skos/core#inScheme> <https://www.ica.org/standards/RiC/vocabularies/recordSetTypes> ;
      <http://www.w3.org/2004/02/skos/core#topConceptOf> <https://www.ica.org/standards/RiC/vocabularies/recordSetTypes> ;
      rdfs:label "item"@en ,
                 "pièce"@fr ,
                 "unidad documental simple"@es .


###  http://lod.ehri-project-test.eu/ontology#OtherLevel
:OtherLevel rdf:type owl:NamedIndividual ,
                     <http://www.w3.org/2004/02/skos/core#Concept> ,
                     <https://www.ica.org/standards/RiC/ontology#RecordSetType> ;
            <http://www.w3.org/2004/02/skos/core#inScheme> <https://www.ica.org/standards/RiC/vocabularies/recordSetTypes> ;
            <http://www.w3.org/2004/02/skos/core#topConceptOf> <https://www.ica.org/standards/RiC/vocabularies/recordSetTypes> ;
            rdfs:label "autre niveau"@fr ,
                       "other level"@en ,
                       "otro nivel"@en .


###  http://lod.ehri-project-test.eu/vocabularies/recordSetTypes#RecordGroup
<http://lod.ehri-project-test.eu/vocabularies/recordSetTypes#RecordGroup> rdf:type owl:NamedIndividual ,
                                                                                   <http://www.w3.org/2004/02/skos/core#Concept> ,
                                                                                   <https://www.ica.org/standards/RiC/ontology#RecordSetType> ;
                                                                          <http://www.w3.org/2004/02/skos/core#inScheme> <https://www.ica.org/standards/RiC/vocabularies/recordSetTypes> ;
                                                                          <http://www.w3.org/2004/02/skos/core#topConceptOf> <https://www.ica.org/standards/RiC/vocabularies/recordSetTypes> ;
                                                                          rdfs:label "groupe d'enregistrement"@fr ,
                                                                                     "record group"@en ,
                                                                                     "unidad documental compuesta"@es .


###  http://lod.ehri-project-test.eu/vocabularies/recordSetTypes#Subcollection
<http://lod.ehri-project-test.eu/vocabularies/recordSetTypes#Subcollection> rdf:type owl:NamedIndividual ,
                                                                                     <http://www.w3.org/2004/02/skos/core#Concept> ,
                                                                                     <https://www.ica.org/standards/RiC/ontology#RecordSetType> ;
                                                                            <http://www.w3.org/2004/02/skos/core#inScheme> <https://www.ica.org/standards/RiC/vocabularies/recordSetTypes> ;
                                                                            <http://www.w3.org/2004/02/skos/core#topConceptOf> <https://www.ica.org/standards/RiC/vocabularies/recordSetTypes> ;
                                                                            rdfs:label "sous-collection"@fr ,
                                                                                       "sub-collection"@en ,
                                                                                       "subcolección"@es .


###  http://lod.ehri-project-test.eu/vocabularies/recordSetTypes#Subfonds
<http://lod.ehri-project-test.eu/vocabularies/recordSetTypes#Subfonds> rdf:type owl:NamedIndividual ,
                                                                                <http://www.w3.org/2004/02/skos/core#Concept> ,
                                                                                <https://www.ica.org/standards/RiC/ontology#RecordSetType> ;
                                                                       <http://www.w3.org/2004/02/skos/core#inScheme> <https://www.ica.org/standards/RiC/vocabularies/recordSetTypes> ;
                                                                       <http://www.w3.org/2004/02/skos/core#topConceptOf> <https://www.ica.org/standards/RiC/vocabularies/recordSetTypes> ;
                                                                       rdfs:label "sous-fonds"@fr ,
                                                                                  "sub-fonds"@en ,
                                                                                  "subfondo"@es .


###  http://lod.ehri-project-test.eu/vocabularies/recordSetTypes#Subgroup
<http://lod.ehri-project-test.eu/vocabularies/recordSetTypes#Subgroup> rdf:type owl:NamedIndividual ,
                                                                                <http://www.w3.org/2004/02/skos/core#Concept> ,
                                                                                <https://www.ica.org/standards/RiC/ontology#RecordSetType> ;
                                                                       <http://www.w3.org/2004/02/skos/core#inScheme> <https://www.ica.org/standards/RiC/vocabularies/recordSetTypes> ;
                                                                       <http://www.w3.org/2004/02/skos/core#topConceptOf> <https://www.ica.org/standards/RiC/vocabularies/recordSetTypes> ;
                                                                       rdfs:label "sous-groupe"@fr ,
                                                                                  "sub-group"@en ,
                                                                                  "subunidad documental compuesta"@es .


###  http://lod.ehri-project-test.eu/vocabularies/recordSetTypes#Subseries
<http://lod.ehri-project-test.eu/vocabularies/recordSetTypes#Subseries> rdf:type owl:NamedIndividual ,
                                                                                 <http://www.w3.org/2004/02/skos/core#Concept> ,
                                                                                 <https://www.ica.org/standards/RiC/ontology#RecordSetType> ;
                                                                        <http://www.w3.org/2004/02/skos/core#inScheme> <https://www.ica.org/standards/RiC/vocabularies/recordSetTypes> ;
                                                                        <http://www.w3.org/2004/02/skos/core#topConceptOf> <https://www.ica.org/standards/RiC/vocabularies/recordSetTypes> ;
                                                                        rdfs:label "sous-série"@fr ,
                                                                                   "sub-series"@en ,
                                                                                   "subserie"@es .


###  Generated by the OWL API (version 5.1.18) https://github.com/owlcs/owlapi/
